src/util/Eqb.v
@@ -23,8 +23,37 @@ Section eqb_prod.
   Qed.
 End eqb_prod.
 
+Section eqb_option.
+  Context {A : Type}.
+  Context {eqbA : Eqb A} {eqbA_ok : Eqb_ok eqbA}.
+
+  #[global] Instance eqb_option : Eqb (option A) :=
+    fun x y => match x, y with
+               | Some a, Some b => eqb a b
+               | None, None => true
+               | _, _ => false
+               end.
+
+  #[global] Instance eqb_option_ok : Eqb_ok eqb_option.
+  Proof.
+    intros [a|] [b|]; cbv [eqb eqb_option]; simpl; try congruence.
+    pose proof (eqb_spec a b) as H. cbv [eqb] in *.
+    destruct (eqbA a b); simpl in H |- *; congruence.
+  Qed.
+End eqb_option.
+
 Lemma eqb_sym {A} {f : Eqb A} {Hok : Eqb_ok f} (a b : A) : eqb a b = eqb b a.
 Proof.
   pose proof (eqb_spec a b) as Hab. pose proof (eqb_spec b a) as Hba.
   destruct (eqb a b), (eqb b a); congruence.
+Qed.
+
+Lemma eqb_map_inj {A B} {fa : Eqb A} {fa_ok : Eqb_ok fa} {fb : Eqb B} {fb_ok : Eqb_ok fb}
+  (g : A -> B) (Hinj : forall a b, g a = g b -> a = b) (a b : A) :
+  eqb (g a) (g b) = eqb a b.
+Proof.
+  pose proof (eqb_spec (g a) (g b)) as Hg. pose proof (eqb_spec a b) as H.
+  destruct (eqb (g a) (g b)), (eqb a b); simpl in Hg, H; try reflexivity.
+  - apply Hinj in Hg. contradiction.
+  - subst b. contradiction.
 Qed.
